Clap/Compiler/Vectors.lean
@@ -8,10 +8,9 @@ open Lean Meta Elab Qq
 
 namespace Clap.Compiler
 
-def getElemVectorOfIdx (coll : Expr) (idx : Nat) : TermElabM Expr := do
-  let_expr Vector _ sz := ← Meta.inferType coll | throwError m!"{coll} must be a Vector."
+def getElemVectorOfIdx (coll : Expr) (len idx : Nat) : TermElabM Expr := do
   let idxQ : Q(Nat) := ToExpr.toExpr idx
-  let szQ : Q(Nat) := sz
+  let szQ : Q(Nat) := mkNatLit len
   let getElemSansProof ← Meta.mkAppM ``GetElem.getElem #[coll, ToExpr.toExpr idx]
   let proof ← Elab.Term.mkTacticMVar q($idxQ < $szQ) (←`(by get_elem_tactic)) .term
   Term.synthesizeSyntheticMVarsNoPostponing
@@ -33,7 +32,7 @@ def mkVecLit (l : Expr) (sz : Expr) : TermElabM Expr := do
 
 def sequenceAsVecExpr (name : Expr) (t : Expr) (len : Nat) : TermElabM Expr := do
   let array ← mkAppM ``List.toArray #[
-    ←mkListLit t (←List.range len |>.mapM (getElemVectorOfIdx name))
+    ←mkListLit t (←List.range len |>.mapM (getElemVectorOfIdx name len))
   ]
   let u ← getDecLevel t
   inferVectorProof (mkAppN (.const ``Vector.mk [u]) #[t, toExpr len, array])
@@ -42,50 +41,80 @@ def sequenceAsVecExpr (name : Expr) (t : Expr) (len : Nat) : TermElabM Expr := d
 --   let t ← inferType e
 --   return t.isAppOf ``Vector
 
-def explodeVector : Sym.Simp.Simproc := fun e ↦ do
-  let t ← inferType e
-  let_expr Vector t sz := t | return .rfl  
-  unless e.isFVar do return .rfl
-  let sz' ← Sym.simp sz
-  match (sz'.getResultExpr sz).nat? with
-  | .none => throwError m!"{sz} does not simplify to ground"
-  | .some n => let explodedVec ← (sequenceAsVecExpr e t n).run'
-               trace[Clap.Compile.simp.kaboom] m!"Exploding:\n{e}\n==>\n{explodedVec}"
-               return .step explodedVec (←Sym.mkEqRefl e)
+lemma abc {α} {vec : Vector α 2} : vec = #v[vec[0], vec[1]] := by
+  rcases vec with ⟨⟨_ | ⟨_, _ | ⟨_, _ | ⟨_, tl⟩⟩⟩⟩, h⟩
+  · cases h
+  · cases h
+  · rfl
+  · cases h
 
--- /--
--- Intended as `↑` in combination with `↓dontExplodeVector`.
+lemma abc' : ∀ {α} {vec : Vector α 2}, vec = #v[vec[0], vec[1]] :=
+  fun {α vec} ↦
+    vec.casesOn fun arr h ↦
+      arr.casesOn
+        (motive := fun x ↦ ∀ (h : x.size = 2), Vector.mk x h = #v[(Vector.mk x h)[0], (Vector.mk x h)[1]])
+        (
+          fun l h ↦
+            l.casesOn
+              (motive := fun x =>
+                ∀ (h : {toList := x : Array _}.size = 2),
+                  Vector.mk { toList := x } h =
+                  #v[(Vector.mk { toList := x } h)[0], (Vector.mk { toList := x } h)[1]])
+              (fun h ↦ h.casesOn
+                         (motive := fun a t ↦
+                           2 = a →
+                           h ≍ t →
+                           Vector.mk { toList := [] } h =
+                           #v[(Vector.mk { toList := [] } h)[0], (Vector.mk { toList := [] } h)[1]])
+              (fun h_1 ↦ False.elim (noConfusion_of_Nat Nat.ctorIdx h_1)) rfl HEq.rfl)
+              (
+                fun head tail ↦
+                  tail.casesOn
+                    (motive := fun x ↦
+                      ∀ (h : { toList := head :: x : Array _}.size = 2),
+                        Vector.mk { toList := head :: x } h =
+                        #v[(Vector.mk { toList := head :: x } h)[0], (Vector.mk { toList := head :: x } h)[1]])
+                    (
+                      fun h =>
+                        h.casesOn
+                          (motive := fun a t ↦
+                            2 = a →
+                            h ≍ t →
+                            Vector.mk { toList := [head] } h =
+                            #v[(Vector.mk { toList := [head] } h)[0], (Vector.mk { toList := [head] } h)[1]])
+                          (fun h_1 ↦
+                            Nat.elimOffset (0 + 1) [].length 1 h_1
+                            fun x ↦ False.elim (noConfusion_of_Nat Nat.ctorIdx x))
+                          rfl
+                          HEq.rfl
+                    )
+                    (
+                      fun head_1 tail h ↦
+                        tail.casesOn (motive := fun x ↦
+                          ∀ (h : { toList := head :: head_1 :: x : Array _ }.size = 2),
+                            Vector.mk { toList := head :: head_1 :: x } h =
+                              #v[(Vector.mk { toList := head :: head_1 :: x } h)[0],
+                                (Vector.mk { toList := head :: head_1 :: x } h)[1]])
+                          (fun h ↦ Eq.refl (Vector.mk { toList := [head, head_1] } h))
+                          (fun head_2 tl h ↦
+                            Eq.casesOn (motive := fun a t ↦
+                              2 = a →
+                                h ≍ t →
+                                  Vector.mk { toList := head :: head_1 :: head_2 :: tl } h =
+                                    #v[(Vector.mk { toList := head :: head_1 :: head_2 :: tl } h)[0],
+                                      (Vector.mk { toList := head :: head_1 :: head_2 :: tl } h)[1]])
+                              h
+                              (fun h_1 ↦
+                                Nat.elimOffset (0 + 1) (head_1 :: head_2 :: tl).length 1 h_1 fun x ↦
+                                  Nat.elimOffset 0 (head_2 :: tl).length 1 x fun x ↦
+                                    False.elim (noConfusion_of_Nat Nat.ctorIdx x))
+                              rfl HEq.rfl)
+                  h)
+              )     
+          h
+        )
+        h
 
--- - `vec : Vector α k ==> #v[vec[0], vec[1], ..., vec[k - 1]]`
--- -/
--- dsimproc_decl explodeVector (_) := fun e ↦ do
---   let t ← inferType e
---   let_expr Vector t sz := t | return .continue
-  
---   if e.isFVar && (←needsExploding e)
---   then match (←Simp.simp sz).1.nat? with
---        | .none => logError m!"{(←Simp.simp sz).1} is not ground"
---                   return .done e
---        | .some n => let explodedVec ← (sequenceAsVecExpr e t n).run'
---                     trace[Clap.Compile.simp.kaboom] m!"Exploding:\n{e}\n==>\n{explodedVec}"
---                     return .done explodedVec
---   else return .continue
-
--- def rejectVectorSansProof (coll e : Expr) : SimpM Simp.DStep := do
---   let_expr Vector _ _ := ← inferType coll | return .continue
---   return .done e
-
--- /--
--- Use with `↓`.
--- -/
--- dsimproc_decl dontExplodeVector (GetElem.getElem _ _ _) := fun e ↦ do
---   let_expr GetElem.getElem _ _ _ _ _ coll _ _ := e | unreachable!
---   if coll.isFVar
---   then
---     rejectVectorSansProof coll e
---   else 
---     return .continue
-  
 /--
 Use with `↓`.
 -/
@@ -93,5 +122,50 @@ def dontExplodeVector : Sym.Simp.Simproc := fun e ↦ do
   let_expr GetElem.getElem _ _ _ _ _ coll _ _ := e | return .rfl
   unless coll.isFVar && (←inferType coll).isAppOf ``Vector do return .rfl
   return .rfl (done := true)
+
+/--
+Use with ↑.
+
+TODO: The proof is not `rfl`. One can prove all of these `by aesop (add cases [Vector, Array, List])`,
+      but I'd rather not lift to `aesop` and build the proof by hand (viz. `abc'` above).
+-/
+def explodeVector : Sym.Simp.Simproc := fun e ↦ do
+  let t ← inferType e
+  let_expr Vector t sz := t | return .rfl
+  unless e.isFVar do return .rfl
+  let sz' ← Sym.simp sz
+  match (sz'.getResultExpr sz).nat? with
+  | .none => throwError m!"{sz} does not simplify to ground.\nExpr:\n{e}"
+  | .some n => let explodedVec ← (sequenceAsVecExpr e t n).run'
+               trace[Clap.Compile.simp.kaboom] m!"Exploding:\n{e}\n==>\n{explodedVec}"
+               return .step explodedVec (←mkSorry (←mkEq e explodedVec) false)
+
+-- /--
+-- TODO: Thought experiment to explode on demand.
+
+-- TODO: The proof is not `rfl`. One can prove all of these `by aesop (add cases [Vector, Array, List])`,
+--       but I'd rather not lift to `aesop` and build the proof by hand (viz. `abc'` above).
+
+-- TODO: Can we share state so that we know which lambda was processed?
+-- -/
+-- def explodeVector' : Sym.Simp.Simproc := fun e ↦ do
+--   let Expr.lam name t body _ := e | return .rfl
+--   let_expr Vector t sz := t | return .rfl
+--   let sz' ← Sym.simp sz
+--   match (sz'.getResultExpr sz).nat? with
+--   | .none => throwError m!"{sz} does not simplify to ground"
+--   | .some n =>
+--     -- It's very tricky to get this right using `(.bvar 0)` in `body`. Would it be... faster?
+--     -- Does remaking the lambda break sharing in `Sym`?
+--     lambdaTelescopeOne! e fun arg body ↦ do
+--       logInfo m!"This.\nbinder[{arg}] in: {body}\nt:{t}\nn:{n}\n"
+--       let explodedVec ← (sequenceAsVecExpr arg t n).run' -- Ideally `(.bvar 0)`.
+--       logInfo m!"exploded: {explodedVec}"
+--       trace[Clap.Compile.simp.kaboom] m!"Exploding:\n{e}\n==>\n{explodedVec}"
+--       let body ← Sym.replaceS body fun e _ ↦ do
+--         if !Sym.isSameExpr e arg then return .none -- Does this even trigger?
+--         return .some explodedVec
+--         -- unless e matches .bvar 0 do return .none -- The enclosing binder.
+--       return .step (←Sym.mkLambdaFVarsS #[arg] body) (←Sym.mkEqRefl e) -- Not this proof.
 
 end Clap.Compiler
